src/External_Facts.v
@@ -3,9 +3,9 @@ Require Import Term ConcreteEvidence StVM Impl_vm Axioms_Io GenStMonad Helpers_V
 Require Import List.
 Import ListNotations.
 
-Axiom build_comp_external' : forall (t : AnnoTerm) (e : EvidenceC) (n : nat) (o : ev_store) (tr:list Ev),
+Axiom copland_compile_external' : forall (t : AnnoTerm) (e : EvidenceC) (n : nat) (o : ev_store) (tr:list Ev),
     runSt 
-      (build_comp t)
+      (copland_compile t)
       {| st_ev := e; st_trace := tr; st_pl := n; st_store := o |} =
     (Some tt,
      {| st_ev := remote_evidence t n e;
@@ -13,7 +13,7 @@ Axiom build_comp_external' : forall (t : AnnoTerm) (e : EvidenceC) (n : nat) (o 
         st_pl :=
           st_pl
             (
-              execSt (build_comp t)
+              execSt (copland_compile t)
                      {| st_ev := e;
                         st_trace := [];
                         st_pl := n;
@@ -21,7 +21,7 @@ Axiom build_comp_external' : forall (t : AnnoTerm) (e : EvidenceC) (n : nat) (o 
         st_store :=
           st_store
             (
-              execSt (build_comp t)
+              execSt (copland_compile t)
                      {| st_ev := e;
                         st_trace := [];
                         st_pl := n;
@@ -29,9 +29,9 @@ Axiom build_comp_external' : forall (t : AnnoTerm) (e : EvidenceC) (n : nat) (o 
      |}).
 
 
-Lemma build_comp_external : forall (t : AnnoTerm) (e : EvidenceC) (n : nat) (o : ev_store),
+Lemma copland_compile_external : forall (t : AnnoTerm) (e : EvidenceC) (n : nat) (o : ev_store),
     well_formed t ->
-    build_comp t {| st_ev := e; st_trace := []; st_pl := n; st_store := o |} =
+    copland_compile t {| st_ev := e; st_trace := []; st_pl := n; st_store := o |} =
     (Some tt,
      {| st_ev := remote_evidence t n e;
         st_trace := remote_trace t n;
@@ -40,7 +40,7 @@ Lemma build_comp_external : forall (t : AnnoTerm) (e : EvidenceC) (n : nat) (o :
           st_store
             (
               execSt
-                (build_comp t)
+                (copland_compile t)
                   {| st_ev := e;
                      st_trace := [];
                      st_pl := n;
@@ -52,7 +52,7 @@ Proof.
   assert (n = st_pl
             (
               execSt
-                (build_comp t)
+                (copland_compile t)
                   {| st_ev := e;
                      st_trace := [];
                      st_pl := n;
@@ -62,15 +62,15 @@ Proof.
     tauto. 
   }
   rewrite H0' at 4.
-  eapply build_comp_external'.
+  eapply copland_compile_external'.
 Defined.
 
 
 
 
-Lemma build_comp_at' : forall (t : AnnoTerm) (e : EvidenceC) (n : nat) (o : ev_store) (tr: list Ev),
+Lemma copland_compile_at' : forall (t : AnnoTerm) (e : EvidenceC) (n : nat) (o : ev_store) (tr: list Ev),
     well_formed t ->
-    build_comp t {| st_ev := e; st_trace := tr; st_pl := n; st_store := o |} =
+    copland_compile t {| st_ev := e; st_trace := tr; st_pl := n; st_store := o |} =
     (Some tt,
      {| st_ev := toRemote t n e;
         st_trace := tr ++ remote_events t n;
@@ -79,7 +79,7 @@ Lemma build_comp_at' : forall (t : AnnoTerm) (e : EvidenceC) (n : nat) (o : ev_s
           st_store
             (
               execSt
-                (build_comp t)
+                (copland_compile t)
                 {| st_ev := e;
                    st_trace := [];
                    st_pl := n;
@@ -92,7 +92,7 @@ Proof.
   
   assert (st_pl
             (execSt
-               (build_comp t)
+               (copland_compile t)
                {| st_ev := e;
                   st_trace := [];
                   st_pl := n;
@@ -100,13 +100,13 @@ Proof.
   eapply pl_immut.
   eauto.
   rewrite <- H0 at 4.
-  eapply build_comp_external'.
+  eapply copland_compile_external'.
 Defined.
 
 
-Lemma build_comp_at : forall (t : AnnoTerm) (e : EvidenceC) (n : nat) (o : ev_store),
+Lemma copland_compile_at : forall (t : AnnoTerm) (e : EvidenceC) (n : nat) (o : ev_store),
     well_formed t ->
-    build_comp t {| st_ev := e; st_trace := []; st_pl := n; st_store := o |} =
+    copland_compile t {| st_ev := e; st_trace := []; st_pl := n; st_store := o |} =
     (Some tt,
      {| st_ev := toRemote t n e;
         st_trace := remote_events t n;
@@ -115,7 +115,7 @@ Lemma build_comp_at : forall (t : AnnoTerm) (e : EvidenceC) (n : nat) (o : ev_st
           st_store
             (
               execSt
-                (build_comp t)
+                (copland_compile t)
                 {| st_ev := e;
                               st_trace := [];
                               st_pl := n;
@@ -125,13 +125,13 @@ Proof.
   intros.
   rewrite at_evidence.
   rewrite at_events.
-  eapply build_comp_external; eauto.
+  eapply copland_compile_external; eauto.
 Defined.
 
-Lemma build_comp_par' :
+Lemma copland_compile_par' :
   forall (t : AnnoTerm) (e : EvidenceC) (n : nat) (o : ev_store) (tr:list Ev),
     well_formed t ->
-    build_comp t {| st_ev := e; st_trace := tr; st_pl := n; st_store := o |} =
+    copland_compile t {| st_ev := e; st_trace := tr; st_pl := n; st_store := o |} =
     (Some tt,
      {|
        st_ev := parallel_vm_thread t n e;
@@ -140,7 +140,7 @@ Lemma build_comp_par' :
        st_store :=
          st_store
            (execSt
-              (build_comp t)
+              (copland_compile t)
               {| st_ev := e;
                  st_trace := [];
                  st_pl := n;
@@ -152,7 +152,7 @@ Proof.
   rewrite par_events.
   assert (st_pl
             (execSt
-               (build_comp t)
+               (copland_compile t)
                {| st_ev := e;
                   st_trace := [];
                   st_pl := n;
@@ -160,13 +160,13 @@ Proof.
   eapply pl_immut.
   eauto.
   rewrite <- H0 at 4.
-  eapply build_comp_external'.
+  eapply copland_compile_external'.
 Defined.
 
-Lemma build_comp_par :
+Lemma copland_compile_par :
   forall (t : AnnoTerm) (e : EvidenceC) (n : nat) (o : ev_store),
     well_formed t ->
-    build_comp t {| st_ev := e; st_trace := []; st_pl := n; st_store := o |} =
+    copland_compile t {| st_ev := e; st_trace := []; st_pl := n; st_store := o |} =
     (Some tt,
      {|
        st_ev := parallel_vm_thread t n e;
@@ -175,7 +175,7 @@ Lemma build_comp_par :
        st_store :=
          st_store
            ( execSt
-               (build_comp t)
+               (copland_compile t)
                 {| st_ev := e;
                    st_trace := [];
                    st_pl := n;
@@ -185,5 +185,5 @@ Proof.
   intros.
   rewrite par_evidence.
   rewrite par_events.
-  eapply build_comp_external; eauto.
+  eapply copland_compile_external; eauto.
 Defined. 
