src/Helpers_VmSemantics.v
@@ -1,256 +1,14 @@
 Require Import MonadVM Impl_vm Term Auto StructTactics MonadVMFacts Maps GenStMonad.
 
-Require Import Coq.Program.Tactics Coq.Program.Equality Lia.
+Require Import Coq.Program.Tactics Coq.Program.Equality.
 
 Set Nested Proofs Allowed.
-
-Lemma hhh : forall t1 t2 a b c d r s,
-    well_formed (abpar r s t1 t2) -> 
-    range t1 = (a,b) ->
-    range t2 = (c,d) ->
-    PeanoNat.Nat.eqb a c = false.
-Proof.
-  intros.
-  assert (fst (range t1) <> fst (range t2)).
-  eapply afaf; eauto.
-  subst''.
-  subst''.
-  simpl in *.
-  rewrite PeanoNat.Nat.eqb_neq in *.
-  tauto.
-Defined.
-
-Lemma faf : forall n,
-    n > 0 -> 
-    n <> n - 1.
-Proof.
-  intros.
-  lia.
-Defined.
-
-Lemma hhhh : forall t1 t2 a b c d r s,
-    well_formed (abpar r s t1 t2) ->
-    range t1 = (a,b) ->
-    range t2 = (c,d) ->
-    PeanoNat.Nat.eqb c (b - 1) = false.
-Proof.
-  intros.
-  inversion H.
-  subst.
-  assert (c = fst (range t2)).
-  {
-    jkjke.
-  }
-
-  assert (a = fst (range t1)).
-  {
-    jkjke.
-  }
-
-  assert (b = snd (range t1)).
-  {
-    jkjk.
-    tauto.
-  }
-
-  assert (d = snd (range t2)).
-  {
-    jkjke.
-  }
-  
-  rewrite H2.
-  rewrite H4.
-  rewrite H9.
-
-  assert (fst (range t2) > 0).
-  {
-    lia.
-  }
-  
-    
-  assert ((fst (range t2)) <> (fst (range t2) - 1)).
-  {
-    eapply faf; eauto.
-  }
-  eapply PeanoNat.Nat.eqb_neq; eauto.
-Defined.
-
-Lemma ppp{A:Type} : forall x:(A*A),
-    x = (fst x, snd x).
-Proof.
-  intros.
-  destruct x.
-  simpl.
-  tauto.
-Defined.
-
-Lemma wf_term_greater : forall t a b,
-    well_formed t ->
-    range t = (a,b) ->
-    b > a.
-Proof.
-  induction t; intros.
-  -
-    destruct a.
-    +
-      simpl in *.
-      inv H.
-      simpl in *.
-      lia.
-    +
-      simpl in *.
-      inv H.
-      simpl in *.
-      lia.
-    +
-      simpl in *.
-      inv H.
-      simpl in *.
-      lia.
-  -
-    simpl in *.
-    subst.
-    inv H.
-    simpl in *.
-    assert (snd (range t) > fst (range t)).
-    eapply IHt.
-    eauto.
-    
-    apply ppp.
-    lia.
-  -
-    inv H.
-    assert (snd (range t1) > fst (range t1)).
-    eapply IHt1.
-    eauto.
-    apply ppp.
-
-    assert (snd (range t2) > fst (range t2)).
-    eapply IHt2.
-    eauto.
-    apply ppp.
-
-    simpl in *.
-    subst.
-
-    simpl in *.
-    lia.
-  -
-    inv H.
-    assert (snd (range t1) > fst (range t1)).
-    eapply IHt1.
-    eauto.
-    apply ppp.
-
-    assert (snd (range t2) > fst (range t2)).
-    eapply IHt2.
-    eauto.
-    apply ppp.
-
-    simpl in *.
-    subst.
-
-    simpl in *.
-    lia.
-  -
-    inv H.
-    assert (snd (range t1) > fst (range t1)).
-    eapply IHt1.
-    eauto.
-    apply ppp.
-
-    assert (snd (range t2) > fst (range t2)).
-    eapply IHt2.
-    eauto.
-    apply ppp.
-
-    simpl in *.
-    subst.
-
-    simpl in *.
-    lia.
-Defined.
-
-Lemma hhhhh : forall t1 t2 a b c d r s,
-    well_formed (abpar r s t1 t2) ->
-    range t1 = (a,b) ->
-    range t2 = (c,d) ->
-    PeanoNat.Nat.eqb (b - 1) (d - 1) = false.
-Proof.
-  intros.
-  inversion H.
-  subst.
-  assert (c = fst (range t2)).
-  {
-    jkjke.
-  }
-
-  assert (a = fst (range t1)).
-  {
-    jkjke.
-  }
-
-  assert (b = snd (range t1)).
-  {
-    jkjk.
-    tauto.
-  }
-
-  assert (d = snd (range t2)).
-  {
-    jkjke.
-  }
-
-
-
-  assert (b <> d).
-  {
-    assert (b = c).
-    {
-      lia.
-    }
-    
-    assert (b > a).
-    {
-      eapply wf_term_greater.
-      apply H6.
-      eauto.
-    }
-
-    assert (d > c).
-    {
-      eapply wf_term_greater; eauto.
-    }
-
-    lia.
-  }
-
-  assert (b > 0).
-  {
-    lia.
-  }
-
-
-  
-
-  assert (d > 0).
-  {
-    assert (d > c).
-    {
-      eapply wf_term_greater; eauto.
-    }
-    lia.
-  }
-
-  eapply PeanoNat.Nat.eqb_neq.
-  lia.
-Defined.
 
 Lemma pl_immut : forall t e tr p o,
     well_formed t ->
     st_pl
       (execSt
-         (build_comp t)
+         (copland_compile t)
          {|
            st_ev := e;
            st_trace := tr;
@@ -263,7 +21,7 @@ Proof.
     destruct a;
       reflexivity.
   -
-    repeat (df; dohtac).
+    repeat (df; dohtac; df).
     reflexivity.
   -
     do_wf_pieces.
@@ -342,9 +100,26 @@ Proof.
       symmetry.
       edestruct IHt1.
       eassumption.
-        jkjk'; eauto.     
+        jkjk'; eauto. 
   -
-    repeat (df; dohtac).
+    repeat (df; dohtac; df; try tauto).
+
+    (*
+
+    (*
+    assert (PeanoNat.Nat.eqb n3 n1 = false /\
+            PeanoNat.Nat.eqb n1 (n4 - 1) = false /\
+            PeanoNat.Nat.eqb (n4 - 1) (n2 - 1) = false) as W by
+          (eapply abpar_store_non_overlap; [apply H | apply Heqr2 | apply Heqr1]);
+      destruct W as [X [Y Z]].
+    rewrite X in *; clear X.
+      rewrite Y in *; clear Y.
+     *)
+    
+
+    htac''.
+
+    
 
     
       
@@ -355,6 +130,8 @@ Proof.
     subst''.
     df.
 
+    
+
 
 
     assert (PeanoNat.Nat.eqb n1 (n4 - 1) = false).
@@ -362,7 +139,8 @@ Proof.
       eapply hhhh; eauto.
     }
     subst''.
-    repeat (df; dohtac).
+    repeat (df; dohtac; try tauto).
+    reflexivity.
 
 
 
@@ -370,9 +148,7 @@ Proof.
     {
       eapply hhhhh; eauto.
     }
-    subst''.
-    repeat (df; dohtac).
-    reflexivity.
+    reflexivity. *)
 Defined.
 
 Ltac do_pl_immut :=
@@ -383,7 +159,7 @@ Ltac do_pl_immut :=
           reflexivity | 
           apply H2] in
       match goal with
-      | [H: build_comp ?t
+      | [H: copland_compile ?t
             {| st_ev := _;
                         st_trace := _;
                         st_pl := ?p;
@@ -427,9 +203,9 @@ Ltac anhl :=
   annogo;
   match goal with
   | [H: well_formed ?a,
-     H2: build_comp ?a _ = _,
-     H3: build_comp ?a _ = _,
-     IH: context[well_formed ?a (*build_comp ?a _ = _ *) -> _] |- _] =>
+     H2: copland_compile ?a _ = _,
+     H3: copland_compile ?a _ = _,
+     IH: context[well_formed ?a (*copland_compile ?a _ = _ *) -> _] |- _] =>
     edestruct IH;
     [apply H | 
      apply H2 | apply H3 | idtac]; clear H2; clear H3;
@@ -438,9 +214,9 @@ Ltac anhl :=
 
 Lemma hihi : forall t e e' e'' x x' y y' p p' p'' o o' o'',
     well_formed t ->
-    build_comp t {| st_ev := e; st_trace := x; st_pl := p; st_store := o |} =
+    copland_compile t {| st_ev := e; st_trace := x; st_pl := p; st_store := o |} =
     (Some tt, {| st_ev := e'; st_trace := x'; st_pl := p'; st_store := o' |}) ->
-    build_comp t {| st_ev := e; st_trace := y; st_pl := p; st_store := o |} =
+    copland_compile t {| st_ev := e; st_trace := y; st_pl := p; st_store := o |} =
     (Some tt, {| st_ev := e''; st_trace := y'; st_pl := p''; st_store := o'' |}) ->
     (e' = e'' /\ p' = p'' /\ o' = o'').
 Proof.
@@ -449,7 +225,7 @@ Proof.
       df; eauto.
   -
     do_wf_pieces.
-    repeat (df; dohtac).
+    repeat (df; dohtac; df).
     tauto.
   -
     do_wf_pieces.
@@ -471,9 +247,10 @@ Proof.
     eauto.   
   -
     do_wf_pieces.
-    repeat (
-        df;
-        dohtac).
+    repeat (df; dohtac; df).
+    tauto.
+
+    (*
 
         assert (PeanoNat.Nat.eqb n3 n1 = false).
     {
@@ -500,7 +277,7 @@ Proof.
     subst''.
     repeat (df; dohtac).
     
-    tauto.
+    tauto. *)
 Defined.
 
 Ltac clear_triv :=
@@ -512,9 +289,9 @@ Ltac dohi'' :=
   annogo;
   let tac Hwf H H' := eapply hihi; [apply Hwf | apply H | apply H'] in
   match goal with
-  | [H : build_comp ?t1 {| st_ev := ?e; st_trace := _; st_pl := ?p; st_store := ?o |} =
+  | [H : copland_compile ?t1 {| st_ev := ?e; st_trace := _; st_pl := ?p; st_store := ?o |} =
          (?opt, {| st_ev := ?e'; st_trace := _; st_pl := ?p'; st_store := ?o' |}),
-         H' : build_comp ?t1 {| st_ev := ?e; st_trace := _; st_pl := ?p; st_store := ?o |} =
+         H' : copland_compile ?t1 {| st_ev := ?e; st_trace := _; st_pl := ?p; st_store := ?o |} =
               (?opt, {| st_ev := ?e''; st_trace := _; st_pl := ?p''; st_store := ?o'' |}),
                 Hwf : well_formed ?t1  |- _] =>
     assert_new_proof_by (e' = e'' /\ p' = p'' /\ o' = o'') ltac:(tac Hwf H H')
@@ -529,8 +306,8 @@ Ltac dohi' :=
   annogo;
   match goal with
   | [H: well_formed ?a, 
-        H2: build_comp ?a _ = _,
-            H3: build_comp ?a _ = _ |- _] =>
+        H2: copland_compile ?a _ = _,
+            H3: copland_compile ?a _ = _ |- _] =>
     edestruct hihi;
     [ (apply H) | 
       repeat dunit; apply H2 |
@@ -562,7 +339,7 @@ Defined.
 
 Lemma always_some : forall t vm_st vm_st' op,
     well_formed t ->
-    build_comp 
+    copland_compile 
       t
       vm_st =
     (op, vm_st') ->
@@ -573,7 +350,7 @@ Proof.
     destruct a;
       try (df; tauto).
   -
-    repeat (df; dohtac).
+    repeat (df; dohtac; df).
     tauto.
   -
     df. 
@@ -590,7 +367,9 @@ Proof.
           df; eauto). 
   -
     do_wf_pieces.
-    repeat (df; dohtac).
+    repeat (df; dohtac; df).
+    tauto.
+    (*
         assert (PeanoNat.Nat.eqb n3 n1 = false).
     {
       eapply hhh; eauto.
@@ -615,12 +394,12 @@ Proof.
     }
     subst''.
     repeat (df; dohtac).
-    tauto.
+    tauto. *)
 Defined.
 
 Ltac do_somett :=
   match goal with
-  | [H: build_comp ?t _ = (?o, _),
+  | [H: copland_compile ?t _ = (?o, _),
         H2: well_formed ?t |- _] =>
     assert_new_proof_by (o = Some tt) ltac:(eapply always_some; [apply H2 | apply H])
   end.
@@ -628,18 +407,18 @@ Ltac do_somett :=
 
 Ltac do_asome := repeat do_somett; clear_triv.
 
-Lemma trace_irrel_store' : forall t tr1 tr1' tr2 e e' p1' p1 o' o,
+Lemma trace_irrel_store : forall t tr1 tr1' tr2 e e' p1' p1 o' o,
     well_formed t ->
-    build_comp t
+    copland_compile t
            {| st_ev := e;  st_trace := tr1; st_pl := p1;  st_store := o  |} =
     (Some tt, {| st_ev := e'; st_trace := tr1'; st_pl := p1'; st_store := o' |}) ->
     
     st_store
-      (execSt (build_comp t)
+      (execSt (copland_compile t)
            {| st_ev := e;  st_trace := tr2; st_pl := p1;  st_store := o  |}) = o'.
 Proof.
   intros.
-  destruct (build_comp t {| st_ev := e; st_trace := tr2; st_pl := p1; st_store := o |}) eqn:ff.
+  destruct (copland_compile t {| st_ev := e; st_trace := tr2; st_pl := p1; st_store := o |}) eqn:ff.
   simpl.
   vmsts.
   simpl.
@@ -650,18 +429,18 @@ Proof.
   tauto.
 Defined.
 
-Lemma trace_irrel_pl' : forall t tr1 tr1' tr2 e e' p1' p1 o' o,
+Lemma trace_irrel_pl : forall t tr1 tr1' tr2 e e' p1' p1 o' o,
     well_formed t ->
-    build_comp t
+    copland_compile t
            {| st_ev := e;  st_trace := tr1; st_pl := p1;  st_store := o  |} =
     (Some tt, {| st_ev := e'; st_trace := tr1'; st_pl := p1'; st_store := o' |}) ->
     
     st_pl
-      (execSt (build_comp t)
+      (execSt (copland_compile t)
            {| st_ev := e;  st_trace := tr2; st_pl := p1;  st_store := o  |}) = p1'.
 Proof.
   intros.
-  destruct (build_comp t {| st_ev := e; st_trace := tr2; st_pl := p1; st_store := o |}) eqn:ff.
+  destruct (copland_compile t {| st_ev := e; st_trace := tr2; st_pl := p1; st_store := o |}) eqn:ff.
   simpl.
   vmsts.
   simpl.
@@ -672,18 +451,18 @@ Proof.
   tauto.
 Defined.
 
-Lemma trace_irrel_ev' : forall t tr1 tr1' tr2 e e' p1' p1 o' o,
+Lemma trace_irrel_ev : forall t tr1 tr1' tr2 e e' p1' p1 o' o,
     well_formed t ->
-    build_comp t
+    copland_compile t
            {| st_ev := e;  st_trace := tr1; st_pl := p1;  st_store := o  |} =
     (Some tt, {| st_ev := e'; st_trace := tr1'; st_pl := p1'; st_store := o' |}) ->
     
     st_ev
-      (execSt (build_comp t)
+      (execSt (copland_compile t)
            {| st_ev := e;  st_trace := tr2; st_pl := p1;  st_store := o  |}) = e'.
 Proof.
   intros.
-  destruct (build_comp t {| st_ev := e; st_trace := tr2; st_pl := p1; st_store := o |}) eqn:ff.
+  destruct (copland_compile t {| st_ev := e; st_trace := tr2; st_pl := p1; st_store := o |}) eqn:ff.
   simpl.
   vmsts.
   simpl.
