src/MonadVM.v
@@ -5,21 +5,19 @@ Author:  Adam Petz, ampetz@ku.edu
 *)
 
 Require Import Term ConcreteEvidence GenStMonad Axioms_Io.
-Require Import Maps.
+Require Import Maps StructTactics.
 
 Require Import List.
 Import ListNotations.
 
-Require Import StructTactics.
-
 Require Export StVM.
 
-Definition VM := St vm_st.
+Definition CVM := St cvm_st.
 
 
 (* VM monad operations *)
 
-Definition put_store_at (n:nat) (e:EvidenceC) : VM unit :=
+Definition put_store_at (n:nat) (e:EvidenceC) : CVM unit :=
   st <- get ;;
      let e' := st_ev st in
      let tr' := st_trace st in
@@ -28,7 +26,7 @@ Definition put_store_at (n:nat) (e:EvidenceC) : VM unit :=
   (*let '{| st_ev := _; st_stack := s; st_trace := tr |} := st in*)
      put (mk_st e' tr' p' (map_set store' n e)).
 
-Definition get_store_at (n:nat) : VM EvidenceC :=
+Definition get_store_at (n:nat) : CVM EvidenceC :=
   st <- get ;;
      let store' := st_store st in
      let maybeEv := map_get store' n in
@@ -37,7 +35,7 @@ Definition get_store_at (n:nat) : VM EvidenceC :=
      | None => failm
      end.
 
-Definition put_ev (e:EvidenceC) : VM unit :=
+Definition put_ev (e:EvidenceC) : CVM unit :=
   st <- get ;;
      let tr' := st_trace st in
      let p' := st_pl st in
@@ -45,28 +43,28 @@ Definition put_ev (e:EvidenceC) : VM unit :=
   (*let '{| st_ev := _; st_stack := s; st_trace := tr |} := st in*)
     put (mk_st e tr' p' store').
 
-Definition get_ev : VM EvidenceC :=
+Definition get_ev : CVM EvidenceC :=
   st <- get ;;
   ret (st_ev st).
 
-Definition get_pl : VM Plc :=
+Definition get_pl : CVM Plc :=
   st <- get ;;
   ret (st_pl st).
 
-Definition modify_evm (f:EvidenceC -> EvidenceC) : VM unit :=
+Definition modify_evm (f:EvidenceC -> EvidenceC) : CVM unit :=
   st <- get ;;
   let '{| st_ev := e; st_trace := tr; st_pl := p; st_store := store |} := st in
   put (mk_st (f e) tr p store).
 
-Definition add_trace (tr':list Ev) : vm_st -> vm_st :=
+Definition add_trace (tr':list Ev) : cvm_st -> cvm_st :=
   fun '{| st_ev := e; st_trace := tr; st_pl := p; st_store := store |} =>
     mk_st e (tr ++ tr') p store.
 
-Definition add_tracem (tr:list Ev) : VM unit :=
+Definition add_tracem (tr:list Ev) : CVM unit :=
   modify (add_trace tr).
 
 
-Definition split_evm (i:nat) (sp1 sp2:SP) (e:EvidenceC) (p:Plc) : VM (EvidenceC*EvidenceC) :=
+Definition split_evm (i:nat) (sp1 sp2:SP) (e:EvidenceC) (p:Plc) : CVM (EvidenceC*EvidenceC) :=
     let e1 := splitEv sp1 e in
     let e2 := splitEv sp2 e in
     add_tracem [Term.split i p] ;;
@@ -74,7 +72,7 @@ Definition split_evm (i:nat) (sp1 sp2:SP) (e:EvidenceC) (p:Plc) : VM (EvidenceC*
 
 (** * Partially-symbolic implementations of IO operations *)
 
-Definition invokeUSM (x:nat) (i:ASP_ID) (l:list Arg) (e:EvidenceC) : VM BS :=
+Definition invokeUSM (x:nat) (i:ASP_ID) (l:list Arg) (e:EvidenceC) : CVM BS :=
   (*e <- get_ev ;; *)
   p <- get_pl ;;
   add_tracem [Term.umeas x p i l];;
@@ -84,7 +82,7 @@ Definition invokeUSM (x:nat) (i:ASP_ID) (l:list Arg) (e:EvidenceC) : VM BS :=
 Definition encodeEv (e:EvidenceC) : BS.
 Admitted.
 
-Definition signEv (x:nat) (e:EvidenceC) : VM BS :=
+Definition signEv (x:nat) (e:EvidenceC) : CVM BS :=
   (* e <- get_ev ;; *)
   p <- get_pl ;;
   add_tracem [Term.sign x p] ;;
@@ -92,18 +90,18 @@ Definition signEv (x:nat) (e:EvidenceC) : VM BS :=
   (*ret (ggc x e)*).
 
 (*
-Definition hashEv (x:nat) (p:Plc) : VM EvidenceC :=
+Definition hashEv (x:nat) (p:Plc) : CVM EvidenceC :=
   e <- get_ev ;;
   add_tracem [Term.hash x p] ;;
   ret (hhc x e).
 *)
 
-Definition copyEv (x:nat) : VM EvidenceC :=
+Definition copyEv (x:nat) : CVM EvidenceC :=
   p <- get_pl ;;
   add_tracem [Term.copy x p] ;;
   get_ev.
 
-Definition do_prim (x:nat) (a:ASP) : VM EvidenceC :=
+Definition do_prim (x:nat) (a:ASP) : CVM EvidenceC :=
   match a with
   | CPY => copyEv x
   | ASPC asp_id args =>
@@ -117,25 +115,25 @@ Definition do_prim (x:nat) (a:ASP) : VM EvidenceC :=
  (* | HSH => hashEv x p  *)
   end.
 
-Definition sendReq (t:AnnoTerm) (q:Plc) (reqi:nat) : VM unit :=
+Definition sendReq (t:AnnoTerm) (q:Plc) (reqi:nat) : CVM unit :=
   p <- get_pl ;;
   e <- get_ev ;;
   put_store_at reqi e ;;
   add_tracem [req reqi p q (unanno t)].
 
-Definition receiveResp (rpyi:nat) (q:Plc) : VM EvidenceC :=
+Definition receiveResp (rpyi:nat) (q:Plc) : CVM EvidenceC :=
   e <- get_store_at rpyi ;;
   p <- get_pl ;;
   add_tracem [rpy (Nat.pred rpyi) p q] ;;
   ret e.
 
-(* Primitive VM Monad operations that require IO Axioms *)
-Definition doRemote (t:AnnoTerm) (q:Plc) (reqi:nat) (rpyi:nat) : VM unit :=
+(* Primitive CVM Monad operations that require IO Axioms *)
+Definition doRemote (t:AnnoTerm) (q:Plc) (reqi:nat) (rpyi:nat) : CVM unit :=
   e <- get_store_at reqi ;;
   add_tracem (remote_events t q) ;;
   put_store_at rpyi (toRemote t q e).
 
-Definition runParThread (t:AnnoTerm) (p:Plc) (loc1:nat) (loc2:nat) : VM (list Ev) :=
+Definition runParThread (t:AnnoTerm) (p:Plc) (loc1:nat) (loc2:nat) : CVM (list Ev) :=
   e <- get_store_at loc1 ;;
   let el := parallel_vm_events t p in
   let e' := parallel_vm_thread t p e in
@@ -143,53 +141,53 @@ Definition runParThread (t:AnnoTerm) (p:Plc) (loc1:nat) (loc2:nat) : VM (list Ev
   put_store_at loc2 e' ;;
   ret el.
 
-Definition runParThreads (t1 t2:AnnoTerm) (p:Plc) (loc_e1 loc_e1' loc_e2 loc_e2':nat) : VM unit :=
+Definition runParThreads (t1 t2:AnnoTerm) (p:Plc) (loc_e1 loc_e1' loc_e2 loc_e2':nat) : CVM unit :=
   el1 <- runParThread t1 p loc_e1 loc_e1' ;;
   el2 <- runParThread t2 p loc_e2 loc_e2' ;;
   add_tracem (shuffled_events el1 el2).
 
-Definition join_seq (n:nat) (p:Plc) (e1:EvidenceC) (e2:EvidenceC) : VM unit :=
+Definition join_seq (n:nat) (p:Plc) (e1:EvidenceC) (e2:EvidenceC) : CVM unit :=
   put_ev (ssc e1 e2) ;;
   add_tracem [Term.join n p].
 
-Definition join_par (n:nat) (p:Plc) (e1:EvidenceC) (e2:EvidenceC) : VM unit :=
+Definition join_par (n:nat) (p:Plc) (e1:EvidenceC) (e2:EvidenceC) : CVM unit :=
   put_ev (ppc e1 e2) ;;
   add_tracem [Term.join n p].
   
 
 (** * Helper functions for Appraisal *)
 
-Definition extractUev (e:EvidenceC) : VM (BS * EvidenceC) :=
+Definition extractUev (e:EvidenceC) : CVM (BS * EvidenceC) :=
   match e with
   | uuc i bs e' => ret (bs,e')
   | _ => failm
   end.
 
-Definition extractSig (e:EvidenceC) : VM (BS * EvidenceC) :=
+Definition extractSig (e:EvidenceC) : CVM (BS * EvidenceC) :=
   match e with
   | ggc bs e' => ret (bs, e')
   | _ => failm
   end.
 
 (*
-Definition extractHsh (e:EvidenceC) : VM (BS * EvidenceC) :=
+Definition extractHsh (e:EvidenceC) : CVM (BS * EvidenceC) :=
   match e with
   | hhc bs e' => ret (bs, e')
   | _ => failm
   end. *)
 
 
-Definition extractComp (e:EvidenceC) : VM (EvidenceC * EvidenceC) :=
+Definition extractComp (e:EvidenceC) : CVM (EvidenceC * EvidenceC) :=
   match e with
   | ssc e1 e2 => ret (e1,e2)
   (*| ppc e1 e2 => ret (e1,e2) *)
   | _ => failm
   end.
 
-Definition checkSig (x:nat) (i:ASP_ID) (e':EvidenceC) (sig:BS) : VM BS :=
+Definition checkSig (x:nat) (i:ASP_ID) (e':EvidenceC) (sig:BS) : CVM BS :=
   invokeUSM x i ([encodeEv e'] ++ [sig] (* ++ args*) ) mtc.
 
-Definition checkUSM (x:nat) (i:ASP_ID) (l:list Arg) (bs:BS) : VM BS :=
+Definition checkUSM (x:nat) (i:ASP_ID) (l:list Arg) (bs:BS) : CVM BS :=
   invokeUSM x i ([bs] ++ l) mtc.
    
 Ltac monad_unfold :=
