src/StVM.v
@@ -11,7 +11,7 @@ Import ListNotations.
 
 (* Specific VM monad state *)
 Definition ev_store := MapC nat EvidenceC.
-Record vm_st : Type := mk_st
+Record cvm_st : Type := mk_st
                          {st_ev:EvidenceC ;
                           st_trace:list Ev ;
                           st_pl:Plc ;
