src/extra/LtacBug.v
@@ -3,7 +3,9 @@ Proof.
   trivial.
 Defined.
 
+(*
 Set Ltac Debug.
+*)
 
 Ltac temp_ltac :=
   match goal with
@@ -14,23 +16,19 @@ Example temp_ex{A:Type} : forall (c:A), c = c -> c = c.
 Proof.
   intros.
   Fail temp_ltac.
-  apply temp with (c:=c).
-  Check temp.
-  eapply temp with (a0:=a).
-​
-Example temp_ex{A:Type} : forall (c:A),  c = c -> c = c.
-Proof.
+  (* Does this evaluate to: apply temp with (c:=c) ? *)
+  (* Intent is as follows: *)
+  apply temp with (a:=c).
+Qed.
 
-​
 Ltac temp_ltac' :=
   match goal with
   | [H: ?b = _ |- _] => apply temp with (a:=b); eauto
   end.
-​
-Example temp_ex{A:Type} : forall (c:A),  c = c -> c = c.
+
+Example temp_ex'{A:Type} : forall (c:A),  c = c -> c = c.
 Proof.
   intros.
-  Fail temp_ltac.
-  (* evaluates to:       apply temp with (c:=c); eauto *)
-  (* should evaluate to: apply temp with (a:=c); eauto *)
   temp_ltac'.
+Qed.
+
