src/extra/Term_examples.v
@@ -1,0 +1,840 @@
+(* Copland terms, events, and annotated terms *)
+
+(* LICENSE NOTICE
+
+Copyright (c) 2018 The MITRE Corporation.
+All Rights Reserved.
+
+This proof script is free software: you can redistribute it and/or
+modify it under the terms of the BSD License as published by the
+University of California.  See license.txt for details. *)
+
+(** This module contains the basic definitions for Copland terms,
+    events, and annotated terms. *)
+
+Require Import PeanoNat Compare_dec Lia.
+Require Import Preamble StructTactics.
+
+Require Import List.
+Import ListNotations.
+
+(** * Terms and Evidence
+
+    A term is either an atomic ASP, a remote call, a sequence of terms
+    with data a dependency, a sequence of terms with no data
+    dependency, or parallel terms. *)
+
+(** [Plc] represents a place. *)
+
+Notation Plc := nat (only parsing).
+Notation ASP_ID := nat (only parsing).
+Notation N_ID := nat (only parsing).
+Notation Arg := nat (only parsing).
+
+Inductive ASP: Set :=
+| CPY: ASP
+| ASPC: ASP_ID -> list Arg -> ASP
+| SIG: ASP
+| HSH: ASP.
+
+Inductive SP: Set :=
+| ALL
+| NONE.
+
+Definition Split: Set := (SP * SP).
+
+Inductive Term: Set :=
+| asp: ASP -> Term
+| att: Plc -> Term -> Term
+| lseq: Term -> Term -> Term
+| bseq: Split -> Term -> Term -> Term
+| bpar: Split -> Term -> Term -> Term.
+
+Definition vc : Term := asp (ASPC 1 []).
+Definition aterm : Term := att 1 vc.
+Definition bterm : Term := att 1 (lseq vc (asp SIG)).
+Definition sig_server : Term := asp (ASPC 2 []).
+Definition cterm : Term := att 2 (lseq sig_server (asp SIG)).
+Definition dterm : Term := lseq cterm bterm.
+Definition os : Term := asp (ASPC 3 [2]).
+Definition eterm : Term := att 3 (lseq os (asp SIG)).
+Definition fterm : Term := lseq eterm dterm.
+
+(** The structure of evidence. *)
+
+Inductive Evidence: Set :=
+| mt: Evidence
+| uu: ASP_ID -> Plc -> Evidence -> Evidence
+| gg: Plc -> Evidence -> Evidence
+| hh: Plc -> Evidence -> Evidence
+| nn: N_ID -> Evidence -> Evidence
+| ss: Evidence -> Evidence -> Evidence
+| pp: Evidence -> Evidence -> Evidence.
+
+Definition splitEv_T (sp:SP) (e:Evidence) : Evidence :=
+  match sp with
+  | ALL => e
+  | NONE => mt
+  end.
+
+Fixpoint eval_asp t p e :=
+  match t with
+  | CPY => e
+  | ASPC i _ => uu i p e
+  | SIG => gg p e
+  | HSH => hh p e
+  end.
+
+(** The evidence associated with a term, a place, and some initial evidence. *)
+
+Fixpoint eval (t:Term) (p:Plc) (e:Evidence) : Evidence :=
+  match t with
+  | asp a => eval_asp a p e
+  | att q t1 => eval t1 q e
+  | lseq t1 t2 => eval t2 p (eval t1 p e)
+  | bseq s t1 t2 => ss (eval t1 p (splitEv_T (fst s) e))
+                       (eval t2 p (splitEv_T (snd s) e)) 
+  | bpar s t1 t2 => pp (eval t1 p (splitEv_T (fst s) e))
+                      (eval t2 p (splitEv_T (snd s) e))
+  end.
+
+(** * Events
+
+    There are events for each kind of action. This includes ASP
+    actions such as measurement or data processing. It also includes
+    control flow actions: a [split] occurs when a thread of control
+    splits, and a [join] occurs when two threads join.  Each event is
+    distinguished using a unique natural number.
+
+ *)
+
+Inductive Ev: Set :=
+| copy: nat -> Plc -> Ev
+| umeas: nat -> Plc -> ASP_ID -> Ev
+| sign: nat -> Plc -> Ev
+| hash: nat -> Plc -> Ev
+| req: nat -> Plc -> Plc -> Term -> Ev
+| rpy: nat -> Plc -> Plc -> Ev 
+| split: nat -> Plc -> Ev
+| join:  nat -> Plc -> Ev.
+
+Definition eq_ev_dec:
+  forall x y: Ev, {x = y} + {x <> y}.
+Proof.
+  intros;
+    repeat decide equality.
+Defined.
+Hint Resolve eq_ev_dec : core.
+
+(** The natural number used to distinguish evidence. *)
+
+Definition ev x :=
+  match x with
+  | copy i _ => i
+  | umeas i _ _  => i
+  | sign i _ => i
+  | hash i _ => i
+  | req i _ _ _ => i
+  | rpy i _ _ => i 
+  | split i _ => i
+  | join i _ => i
+  end.
+
+(** Events are used in a manner that ensures that
+[[
+    forall e0 e1, ev e0 = ev e1 -> e0 = e1.
+]]
+See Lemma [events_injective].
+ *)
+
+
+Definition asp_event i x p :=
+  match x with
+  | CPY => copy i p
+  | ASPC id _ => umeas i p id
+  | SIG => sign i p
+  | HSH => hash i p
+  end.
+
+
+(** * Annotated Terms
+
+    Annotated terms are used to ensure that each distinct event has a
+    distinct natural number.  To do so, each term is annotated by a
+    pair of numbers called a range.  Let [(i, k)] be the label for
+    term [t].  The labels will be chosen to have the property such
+    that for each event in the set of events associated with term [t],
+    its number [j] will be in the range [i <= j < k].  *)
+
+Definition Range: Set := nat * nat.
+
+Inductive AnnoTerm: Set :=
+| aasp: Range -> ASP -> AnnoTerm
+| aatt: Range -> Plc -> AnnoTerm -> AnnoTerm
+| alseq: Range -> AnnoTerm -> AnnoTerm -> AnnoTerm
+| abseq: Range -> Split -> AnnoTerm -> AnnoTerm -> AnnoTerm
+| abpar: Range -> Split -> AnnoTerm -> AnnoTerm -> AnnoTerm.
+
+(** The number of events associated with a term.  The branching terms
+add a split and a join to the events of their subterms. Similarly, the
+remote calls add a request and receive to the events of their subterm.
+*)
+
+Fixpoint esize t :=
+  match t with
+  | aasp _ _ => 1
+  | aatt _ _ t1 => 2 + esize t1
+  | alseq _ t1 t2 => esize t1 + esize t2
+  | abseq _ _ t1 t2 => 2 + esize t1 + esize t2
+  | abpar _ _ t1 t2 => 2 + esize t1 + esize t2
+  end.
+
+Definition range x :=
+  match x with
+  | aasp r _ => r
+  | aatt r _ _ => r
+  | alseq r _ _ => r
+  | abseq r _ _ _ => r
+  | abpar r _ _ _ => r
+  end.
+
+(** This function annotates a term.  It feeds a natural number
+    throughout the computation so as to ensure each event has a unique
+    natural number. *)
+
+Fixpoint anno (t: Term) i: nat * AnnoTerm :=
+  match t with
+  | asp x => (S i, aasp (i, S i) x)
+  | att p x =>
+    let (j, a) := anno x (S i) in
+    (S j, aatt (i, S j) p a)
+  | lseq x y =>
+    let (j, a) := anno x i in
+    let (k, b) := anno y j in
+    (k, alseq (i, k) a b)
+  | bseq s x y =>
+    let (j, a) := anno x (S i) in
+    let (k, b) := anno y j in
+    (S k, abseq (i, S k) s a b)
+  | bpar s x y =>
+    let (j, a) := anno x (S i) in
+    let (k, b) := anno y j in
+    (S k, abpar (i, S k) s a b)
+  end.
+
+Lemma anno_mono : forall t i j t',
+  anno t i = (j, t') ->
+  j > i.
+Proof.
+  induction t; intros.
+  - destruct a;
+      try (unfold anno in *;
+           inv H;
+           lia).
+  - simpl in *.
+    break_let.
+    invc H.
+    assert (n0 > (S i)).
+    eauto.
+    lia.
+  -
+    simpl in *.
+    repeat break_let.
+    invc H.
+    assert (n > i); eauto.
+    assert (j > n); eauto.
+    lia.
+  - simpl in *.
+    repeat break_let.
+    invc H.
+    assert (n > (S i)); eauto.
+    assert (n0 > n); eauto.
+    lia.
+  -
+    simpl in *.
+    repeat break_let.
+    invc H.
+    assert (n > (S i)); eauto.
+    assert (n0 > n); eauto.
+    lia.
+Defined.
+
+Lemma anno_range:
+  forall x i,
+    range (snd (anno x i)) = (i, fst (anno x i)).
+Proof.
+  induction x; intros; simpl; auto;
+    repeat expand_let_pairs;
+    simpl; auto.
+Qed.
+
+Definition annotated x :=
+  snd (anno x 0).
+
+Lemma pairsinv : forall (a a' b b':nat),
+    a <> a' -> (a,b) <> (a',b').
+Proof.
+  intros.
+  congruence.
+Defined.
+
+Lemma afaf : forall i k s a b t' n,
+    (abpar (i, k) s a b) = snd (anno t' n)(*(bpar s x y)*) ->
+    (fst (range a)) <> (fst (range b)).
+Proof.
+  intros.
+  destruct t';
+    cbn in *;
+    repeat (break_let);
+    simpl in *;
+    try solve_by_inversion.
+
+
+(*
+  unfold annotated in *.
+  cbn in *.
+  remember (anno t'1 (S n)) as oo.
+  destruct oo.
+  remember (anno t'2 n0) as oo.
+  destruct oo.
+  
+  simpl in *.
+  repeat break_let.
+ *)
+  
+  inv H.
+  assert (n0 > (S n)).
+  eapply anno_mono; eauto.
+  assert (n1 > n0).
+  eapply anno_mono; eauto.
+  assert ( range (snd (anno t'1 (S n))) = ((S n), fst (anno t'1 (S n)))).
+  eapply anno_range; eauto.
+  subst.
+  rewrite Heqp in H2.
+  simpl in *.
+
+  assert ( range (snd (anno t'2 n0)) = (n0, fst (anno t'2 n0))).
+  eapply anno_range; eauto.
+  rewrite Heqp0 in H3.
+  simpl in *.
+  rewrite H2.
+  rewrite H3.
+  simpl.
+  lia.
+Defined.
+
+Fixpoint unanno a :=
+  match a with
+  | aasp _ a => asp a
+  | aatt _ p t => att p (unanno t)
+  | alseq _ a1 a2 => lseq (unanno a1) (unanno a2)
+                         
+  | abseq _ spl a1 a2 => bseq spl (unanno a1) (unanno a2) 
+  | abpar _ spl a1 a2 => bpar spl (unanno a1) (unanno a2)
+  end.
+
+(** This predicate determines if an annotated term is well formed,
+    that is if its ranges correctly capture the relations between a
+    term and its associated events. *)
+
+Inductive well_formed: AnnoTerm -> Prop :=
+| wf_asp: forall r x,
+    snd r = S (fst r) ->
+    well_formed (aasp r x)
+| wf_att: forall r p x,
+    well_formed x ->
+    S (fst r) = fst (range x) ->
+    snd r = S (snd (range x)) ->
+    well_formed (aatt r p x)
+| wf_lseq: forall r x y,
+    well_formed x -> well_formed y ->
+    fst r = fst (range x) ->
+    snd (range x) = fst (range y) ->
+    snd r = snd (range y) ->
+    well_formed (alseq r x y)
+| wf_bseq: forall r s x y,
+    well_formed x -> well_formed y ->
+    S (fst r) = fst (range x) ->
+    snd (range x) = fst (range y) ->
+    snd r = S (snd (range y)) ->
+    well_formed (abseq r s x y)
+| wf_bpar: forall r s x y,
+    well_formed x -> well_formed y ->
+    S (fst r) = fst (range x) ->
+    snd (range x) = fst (range y) ->
+    snd r = S (snd (range y)) ->
+    well_formed (abpar r s x y).
+Hint Constructors well_formed : core.
+
+Lemma well_formed_range:
+  forall t,
+    well_formed t ->
+    snd (range t) = fst (range t) + esize t.
+Proof.
+  induction t; intros; simpl; inv H; simpl.
+  - rewrite Nat.add_1_r; auto.
+  - apply IHt in H3; lia.
+  - apply IHt1 in H3.
+    apply IHt2 in H4.
+    lia.
+  - apply IHt1 in H4.
+    apply IHt2 in H5.
+    lia.
+  - apply IHt1 in H4.
+    apply IHt2 in H5.
+    lia.
+Qed.
+
+Lemma anno_well_formed:
+  forall t i,
+    well_formed (snd (anno t i)).
+Proof.
+  induction t; intros; simpl; auto.
+  - repeat expand_let_pairs.
+    simpl.
+    apply wf_att; simpl; auto;
+      rewrite anno_range; simpl; reflexivity.
+  - repeat expand_let_pairs.
+    simpl.
+    apply wf_lseq; simpl; auto;
+      repeat rewrite anno_range; simpl;
+        reflexivity.
+  - repeat expand_let_pairs; simpl.
+    apply wf_bseq; simpl; auto;
+      repeat rewrite anno_range; simpl;
+        reflexivity.
+  - repeat expand_let_pairs; simpl.
+    apply wf_bpar; simpl; auto;
+      repeat rewrite anno_range; simpl;
+        reflexivity.
+Qed.
+
+(** Eval for annotated terms. *)
+
+Fixpoint aeval t p e :=
+  match t with
+  | aasp _ x => eval (asp x) p e
+  | aatt _ q x => aeval x q e
+  | alseq _ t1 t2 => aeval t2 p (aeval t1 p e)
+  | abseq _ s t1 t2 => ss (aeval t1 p ((splitEv_T (fst s)) e))
+                         (aeval t2 p ((splitEv_T (snd s)) e)) 
+  | abpar _ s t1 t2 => pp (aeval t1 p ((splitEv_T (fst s)) e))
+                         (aeval t2 p ((splitEv_T (snd s)) e)) 
+  end. 
+
+Lemma eval_aeval:
+  forall t p e i,
+    eval t p e = aeval (snd (anno t i)) p e.
+Proof.
+  induction t; intros; simpl; auto.
+  - repeat expand_let_pairs; simpl;
+      rewrite <- IHt; auto.
+  - repeat expand_let_pairs.
+    simpl.
+    rewrite <- IHt1.
+    rewrite <- IHt2; auto.
+  - repeat expand_let_pairs.
+    simpl.
+    rewrite <- IHt1.
+    rewrite <- IHt2; auto.
+    - repeat expand_let_pairs.
+    simpl.
+    rewrite <- IHt1.
+    rewrite <- IHt2; auto.
+Qed.
+
+(** This predicate specifies when a term, a place, and some initial
+    evidence is related to an event.  In other words, it specifies the
+    set of events associated with a term, a place, and some initial
+    evidence. *)
+
+Inductive events: AnnoTerm -> Plc -> Ev -> Prop :=
+| evtscpy:
+    forall r i p,
+      fst r = i ->
+      events (aasp r CPY) p (copy i p)
+| evtsusm:
+    forall i id args r p,
+      fst r = i ->
+      events (aasp r (ASPC id args)) p (umeas i p id)
+| evtssig:
+    forall r i p,
+      fst r = i ->
+      events (aasp r SIG) p (sign i p) 
+| evtshsh:
+    forall r i p,
+      fst r = i ->
+      events (aasp r HSH) p (hash i p)
+
+| evtsattreq:
+    forall r q t i p,
+      fst r = i ->
+      events (aatt r q t) p (req i p q (unanno t))
+| evtsatt:
+    forall r q t ev p,
+      events t q ev ->
+      events (aatt r q t) p ev
+| evtsattrpy:
+    forall r q t i p,
+      snd r = S i ->
+      events (aatt r q t) p (rpy i p q)
+| evtslseql:
+    forall r t1 t2 ev p,
+      events t1 p ev ->
+      events (alseq r t1 t2) p ev
+| evtslseqr:
+    forall r t1 t2 ev p,
+      events t2 p ev ->
+      events (alseq r t1 t2) p ev
+| evtsbseqsplit:
+    forall r i s t1 t2 p,
+      fst r = i ->
+      events (abseq r s t1 t2) p
+             (split i p)
+| evtsbseql:
+    forall r s t1 t2 ev p,
+      events t1 p ev ->
+      events (abseq r s t1 t2) p ev
+| evtsbseqr:
+    forall r s t1 t2 ev p,
+      events t2 p ev ->
+      events (abseq r s t1 t2) p ev
+| evtsbseqjoin:
+    forall r i s t1 t2 p,
+      snd r = S i ->
+      events (abseq r s t1 t2) p
+             (join i p)
+| evtsbparsplit:
+    forall r i s t1 t2 p,
+      fst r = i ->
+      events (abpar r s t1 t2) p
+             (split i p)
+| evtsbparl:
+    forall r s t1 t2 ev p,
+      events t1 p ev ->
+      events (abpar r s t1 t2) p ev
+| evtsbparr:
+    forall r s t1 t2 ev p,
+      events t2 p ev ->
+      events (abpar r s t1 t2) p ev
+| evtsbparjoin:
+    forall r i s t1 t2 p,
+      snd r = S i ->
+      events (abpar r s t1 t2) p
+             (join i p).
+Hint Constructors events : core.
+
+Lemma events_range:
+  forall t v p,
+    well_formed t ->
+    events t p v ->
+    fst (range t) <= ev v < snd (range t).
+Proof.
+  
+  intros.
+  pose proof H as G.
+  apply well_formed_range in G.
+  rewrite G.
+  clear G.
+  induction H0; inv H; simpl in *; auto; try lia.
+  - apply IHevents in H4; lia.
+  - Check well_formed_range.
+
+    apply well_formed_range in H4; lia.
+  - apply IHevents in H4; lia.
+  - apply IHevents in H5.
+    apply well_formed_range in H4.
+    lia.
+  - apply IHevents in H5; lia.
+  - apply IHevents in H6.
+    apply well_formed_range in H5.
+    lia.
+  - apply well_formed_range in H5.
+    apply well_formed_range in H6.
+    lia.
+  - apply IHevents in H5; lia.
+  - apply IHevents in H6.
+    apply well_formed_range in H5.
+    lia.
+  - apply well_formed_range in H5.
+    apply well_formed_range in H6.
+    lia.
+Qed.
+
+Lemma at_range:
+  forall x r i,
+    S (fst r) = fst x ->
+    snd r = S (snd x) ->
+    fst r <= i < snd r ->
+    i = fst r \/
+    fst x <= i < snd x \/
+    i = snd x.
+Proof.
+  intros.
+  pose proof lt_dec i (S (fst r)) as G.
+  destruct G as [G|G]; [left; lia| right].
+  pose proof lt_dec i (snd x) as F.
+  destruct F as [F|F]; [left; lia| right].
+  lia.
+Qed.
+
+Lemma lin_range:
+  forall x y i,
+    snd x = fst y ->
+    fst x <= i < snd y ->
+    fst x <= i < snd x \/
+    fst y <= i < snd y.
+Proof.
+  intros.
+  pose proof lt_dec i (snd x) as G.
+  destruct G; lia.
+Qed.
+
+Lemma bra_range:
+  forall x y r i,
+    S (fst r) = fst x ->
+    snd x = fst y ->
+    snd r = S (snd y) ->
+    fst r <= i < snd r ->
+    i = fst r \/
+    fst x <= i < snd x \/
+    fst y <= i < snd y \/
+    i = snd y.
+Proof.
+  intros.
+  pose proof lt_dec i (S (fst r)) as G.
+  destruct G as [G|G]; [left; lia| right].
+  pose proof lt_dec i (snd x) as F.
+  destruct F as [F|F]; [left; lia| right].
+  pose proof lt_dec i (snd y) as E.
+  destruct E; lia.
+Qed.
+
+(** Properties of events. *)
+
+Lemma events_range_event:
+  forall t p i,
+    well_formed t ->
+    fst (range t) <= i < snd (range t) ->
+    exists v, events t p v /\ ev v = i.
+Proof.
+  intros t p i H; revert i; revert p.
+  induction H; intros; simpl in *.
+  - destruct x; eapply ex_intro; split; auto;
+      destruct r as [j k]; simpl in *; lia.
+  - eapply at_range in H2; eauto.
+    repeat destruct_disjunct; subst.
+    + eapply ex_intro; split; auto.
+    + apply IHwell_formed with (p:=p) in H2.
+      destruct H2 as [v].
+      destruct H2; subst.
+      exists v; split; auto.
+    + eapply ex_intro; split.
+      apply evtsattrpy; auto.
+      * rewrite H1; auto.
+      * simpl; auto.
+  - apply lin_range with (i:=i) in H2; eauto.
+    destruct H2.
+    + apply IHwell_formed1 with (p:=p) in H2; auto.
+      destruct H2 as [v]; destruct H2; subst.
+      exists v; split; auto.
+    + apply IHwell_formed2 with (p:=p) in H2; auto.
+      destruct H2 as [v]; destruct H2; subst.
+      exists v; split; auto.
+    + lia.
+  - apply bra_range with (i:=i) (r:=r) in H2; eauto.
+    repeat destruct_disjunct; subst.
+    + eapply ex_intro; split; auto.
+    + apply IHwell_formed1 with (p:=p) in H2.
+      destruct H2 as [v]; destruct H2; subst.
+      exists v; split; auto.
+    + apply IHwell_formed2 with (p:=p) in H2.
+      destruct H2 as [v]; destruct H2; subst.
+      exists v; split; auto.
+    + eapply ex_intro; split.
+      * apply evtsbseqjoin; auto.
+        rewrite H3; auto.
+      * simpl; auto.
+  - apply bra_range with (i:=i) (r:=r) in H2; eauto.
+    repeat destruct_disjunct; subst.
+    + eapply ex_intro; split; auto.
+    + apply IHwell_formed1 with (p:=p) in H2.
+      destruct H2 as [v]; destruct H2; subst.
+      exists v; split; auto.
+    + apply IHwell_formed2 with (p:=p) in H2.
+      destruct H2 as [v]; destruct H2; subst.
+      exists v; split; auto.
+    + eapply ex_intro; split.
+      * apply evtsbparjoin; auto.
+        rewrite H3; auto.
+      * simpl; auto.
+Qed.
+
+Ltac events_event_range :=
+  repeat match goal with
+         | [ H: events _ _ _ |- _ ] =>
+           apply events_range in H; auto
+         end; lia.
+
+Lemma events_injective:
+  forall t p v1 v2,
+    well_formed t ->
+    events t p v1 ->
+    events t p v2 ->
+    ev v1 = ev v2 ->
+    v1 = v2.
+Proof.
+  intros t p v1 v2 H; revert v2; revert v1;
+    revert p.
+  induction H; intros.
+  - inv H0; inv H1; auto.
+  - pose proof H as G.
+    apply well_formed_range in G.
+    inv H2; inv H3; simpl in *; subst; auto.
+    + events_event_range.
+    + events_event_range.
+    + events_event_range.
+    + eapply IHwell_formed in H11; eauto.
+    + events_event_range.
+    + events_event_range.
+    + events_event_range.
+  - pose proof H as G.
+    pose proof H0 as G0.
+    apply well_formed_range in G.
+    apply well_formed_range in G0.
+    inv H4; inv H5; simpl in *; auto.
+    + eapply IHwell_formed1 in H13; eauto.
+    + events_event_range.
+    + events_event_range.
+    + eapply IHwell_formed2 in H13; eauto.
+  - pose proof H as G.
+    pose proof H0 as G0.
+    apply well_formed_range in G.
+    apply well_formed_range in G0.
+    inv H4; inv H5; simpl in *; subst; auto.
+    + events_event_range.
+    + events_event_range.
+    + events_event_range.
+    + events_event_range.
+    + eapply IHwell_formed1 in H13; eauto.
+    + events_event_range.
+    + events_event_range.
+    + events_event_range.
+    + events_event_range.
+    + eapply IHwell_formed2 in H13; eauto.
+    + events_event_range.
+    + events_event_range.
+    + events_event_range.
+    + events_event_range.
+  - pose proof H as G.
+    pose proof H0 as G0.
+    apply well_formed_range in G.
+    apply well_formed_range in G0.
+    inv H4; inv H5; simpl in *; subst; auto.
+    + events_event_range.
+    + events_event_range.
+    + events_event_range.
+    + events_event_range.
+    + eapply IHwell_formed1 in H13; eauto.
+    + events_event_range.
+    + events_event_range.
+    + events_event_range.
+    + events_event_range.
+    + eapply IHwell_formed2 in H13; eauto.
+    + events_event_range.
+    + events_event_range.
+    + events_event_range.
+    + events_event_range.
+Qed.
+
+
+
+
+
+
+
+
+Inductive splitEv_T_R : SP -> Evidence -> Evidence -> Prop :=
+| spAll: forall e, splitEv_T_R ALL e e
+| spNone: forall e, splitEv_T_R NONE e mt.
+
+Inductive evalR : Term -> Plc -> Evidence -> Evidence -> Prop :=
+| evalR_asp: forall a p e,
+    evalR (asp a) p e (eval_asp a p e)
+| evalR_att: forall t1 q e e' p,
+    evalR t1 q e e' ->
+    evalR (att q t1) p e e'
+| evalR_lseq: forall t1 t2 p e e' e'',
+    evalR t1 p e e' ->
+    evalR t2 p e' e'' ->
+    evalR (lseq t1 t2) p e e''
+| evalR_bseq: forall s e e1 e2 e1' e2' p t1 t2,
+    splitEv_T_R (fst s) e e1 ->
+    splitEv_T_R (snd s) e e2 ->
+    evalR t1 p e1 e1' ->
+    evalR t2 p e2 e2' ->
+    evalR (bseq s t1 t2) p e (ss e1' e2')
+| evalR_bpar: forall s e e1 e2 e1' e2' p t1 t2,
+    splitEv_T_R (fst s) e e1 ->
+    splitEv_T_R (snd s) e e2 ->
+    evalR t1 p e1 e1' ->
+    evalR t2 p e2 e2' ->
+    evalR (bpar s t1 t2) p e (pp e1' e2').
+
+Lemma eval_iff_evalR: forall t p e e',
+    evalR t p e e' <-> eval t p e = e'.
+Proof.
+  split.
+  - (* -> case *)
+    intros.
+    generalize dependent p.
+    generalize dependent e.
+    generalize dependent e'.
+
+    induction t; intros.
+    + destruct a; try (inv H; reflexivity).
+    + inv H. simpl.
+      eauto.
+    + inv H.
+      assert (eval t1 p e = e'0).
+      eauto.
+      subst.
+      simpl.
+      eauto.
+    + inv H.
+      assert (eval t1 p e1 = e1') by eauto.
+      assert (eval t2 p e2 = e2') by eauto.
+      simpl.
+      destruct s. simpl.
+      destruct s; destruct s0;
+        try (simpl; subst; inv H3; inv H4; reflexivity).
+    + inv H.
+      assert (eval t1 p e1 = e1') by eauto.
+      assert (eval t2 p e2 = e2') by eauto.
+      simpl.
+      destruct s. simpl.
+      destruct s; destruct s0;
+        try (simpl; subst; inv H3; inv H4; reflexivity).
+  - (* <- case *)
+    intros.
+    generalize dependent p.
+    generalize dependent e.
+    generalize dependent e'.
+
+    induction t; intros.
+    + inv H.
+      destruct a; try econstructor.
+    + inv H.
+      simpl.
+      econstructor.
+      eauto.
+    + econstructor; eauto.
+    + destruct s.
+      simpl in H.
+      destruct s; destruct s0; simpl in *; subst;
+        econstructor; (try simpl); eauto; try (econstructor).
+    + destruct s.
+      simpl in H.
+      destruct s; destruct s0; simpl in *; subst;
+        econstructor; (try simpl); eauto; try (econstructor).
+Defined.
